src/study/Nemonuri.Study.CSharpSyntaxRewriter2.Modifier2/Nemonuri.StratifiedNodes.Nodes.Base.Members.fst
@@ -1,0 +1,66 @@
+module Nemonuri.StratifiedNodes.Nodes.Base.Members
+
+module L = FStar.List.Tot
+module I = Nemonuri.StratifiedNodes.Internals
+module T = Nemonuri.StratifiedNodes.Nodes.Base.Types
+module Math = FStar.Math.Lib
+open FStar.Classical.Sugar
+
+//--- (T.node t) members ---
+let get_level #t (node:T.node t) 
+  : Pure pos True (ensures fun r -> (r = (I.get_level node.internal)))
+  = 
+  node.level
+
+let get_value #t (node:T.node t) : Tot t = node.internal.value
+//---|
+
+//--- (T.node_list t) private members ---
+private let rec get_list_level_impl #t (l:T.node_list t) : Tot nat =
+  match l with
+  | [] -> 0
+  | hd::tl -> Math.max (get_level hd) (get_list_level_impl tl)
+//---|
+
+//--- (T.node_list t) propositions ---
+let list_level_is_greater_or_equal_than_element_level 
+  (t:eqtype) (l:T.node_list t) 
+  : prop =
+  (forall (node:T.node t). 
+    (L.contains node l) ==> ((get_level node) <= get_list_level_impl l))
+//---|
+
+//--- (T.node_list t) lemmas ---
+private let rec lemma_list_level_is_greater_or_equal_than_element_level_for_cons
+  (t:eqtype) (n:T.node t) (l:T.node_list t)
+  : Lemma 
+    (requires L.contains n l)
+    (ensures (
+      ((get_level n) <= get_list_level_impl l)
+    ))
+    (decreases l)
+  =
+  let hd::tl = l in
+  if (hd = n) then ()
+  else 
+    lemma_list_level_is_greater_or_equal_than_element_level_for_cons t n tl
+
+let lemma_list_level_is_greater_or_equal_than_element_level (t:eqtype) (l:T.node_list t)
+  : Lemma
+    (ensures (
+      list_level_is_greater_or_equal_than_element_level t l
+    ))
+  = 
+  introduce forall (it_node:T.node t{ L.contains it_node l }). 
+    ((get_level it_node) <= get_list_level_impl l) with (
+      lemma_list_level_is_greater_or_equal_than_element_level_for_cons t it_node l
+    )
+//---|
+
+//--- (T.node_list t) members ---
+let get_list_level #t (l:T.node_list t) 
+  : Pure nat True (ensures fun _ -> list_level_is_greater_or_equal_than_element_level t l) =
+  lemma_list_level_is_greater_or_equal_than_element_level t l;
+  get_list_level_impl l
+
+//---|
