src/study/Nemonuri.Study.CSharpSyntaxRewriter2.Modifier2/Nemonuri.StratifiedNodes.Nodes.Base.Types.fst
@@ -1,0 +1,14 @@
+module Nemonuri.StratifiedNodes.Nodes.Base.Types
+
+module L = FStar.List.Tot
+module I = Nemonuri.StratifiedNodes.Internals
+
+//--- type definitions ---
+type node (t:eqtype) =
+  | SNode : 
+      level:pos ->
+      internal:(I.node_internal t level) ->
+      node t
+
+let node_list (t:eqtype) = list (node t)
+//---|
