src/study/Nemonuri.Study.CSharpSyntaxRewriter2.Modifier2/Nemonuri.StratifiedNodes.Nodes.Base.fst
@@ -1,0 +1,4 @@
+module Nemonuri.StratifiedNodes.Nodes.Base
+
+include Nemonuri.StratifiedNodes.Nodes.Base.Types
+include Nemonuri.StratifiedNodes.Nodes.Base.Members
