src/study/Nemonuri.Study.CSharpSyntaxRewriter2.Modifier2/Nemonuri.StratifiedNodes.Nodes.Bijections.ToNode.fst
@@ -1,0 +1,46 @@
+module Nemonuri.StratifiedNodes.Nodes.Bijections.ToNode
+
+module I = Nemonuri.StratifiedNodes.Internals
+module Base = Nemonuri.StratifiedNodes.Nodes.Base
+open Nemonuri.StratifiedNodes.Nodes.Base.Members
+
+//--- private theory members ---
+private let to_node_impl #t #level (node_internal:I.node_internal t level) : Tot (Base.node t) =
+  Base.SNode level node_internal
+
+private let to_node_inverse_impl #t (nd:Base.node t) : Tot (I.node_internal t (get_level nd)) =
+  nd.internal
+//---|
+
+//--- propositions ---
+let applying_to_node_inverse_after_to_node_is_identity 
+  #t #node_internal_level (node_internal:I.node_internal t node_internal_level) : prop =
+  to_node_inverse_impl (to_node_impl node_internal) == node_internal
+
+let applying_to_node_after_to_node_inverse_is_identity
+  #t (node:Base.node t) : prop =
+  to_node_impl (to_node_inverse_impl node) == node
+
+let to_node_is_bijection (t:eqtype) : prop =
+  (forall (node_internal_level:pos) (node_internal:I.node_internal t node_internal_level).
+    applying_to_node_inverse_after_to_node_is_identity node_internal) /\
+  (forall (node:Base.node t). applying_to_node_after_to_node_inverse_is_identity node)
+//---|
+
+//--- lemma ---
+let lemma_to_node_is_bijection (t:eqtype)
+  : Lemma (ensures to_node_is_bijection t) =
+  ()
+//---|
+
+//--- theory members ---
+let to_node #t #level (node_internal:I.node_internal t level)
+  : Pure (Base.node t) True (ensures fun _ -> to_node_is_bijection t) =
+  lemma_to_node_is_bijection t;
+  to_node_impl node_internal
+
+let to_node_inverse #t (node:Base.node t)
+  : Pure (I.node_internal t (get_level node)) True (ensures fun _ -> to_node_is_bijection t) =
+  lemma_to_node_is_bijection t;
+  to_node_inverse_impl node
+//---|
