src/study/Nemonuri.Study.CSharpSyntaxRewriter2.Modifier2/Nemonuri.StratifiedNodes.Nodes.Bijections.ToNodeList.fst
@@ -1,0 +1,29 @@
+module Nemonuri.StratifiedNodes.Nodes.Bijections.ToNodeList
+
+module I = Nemonuri.StratifiedNodes.Internals
+module Base = Nemonuri.StratifiedNodes.Nodes.Base
+module ToNode = Nemonuri.StratifiedNodes.Nodes.Bijections.ToNode
+open Nemonuri.StratifiedNodes.Nodes.Bijections.ToNode
+open Nemonuri.StratifiedNodes.Nodes.Base.Members
+
+
+//--- private theory members ---
+private let to_node_list_impl #t #max_level 
+  (node_list_internal:I.node_list_internal t max_level) 
+  : Tot (Base.node_list t) =
+  I.select node_list_internal (fun ni -> to_node ni)  
+
+private let rec to_node_list_inverse_impl
+  #t (l:Base.node_list t)
+  : Tot (I.node_list_internal t (get_list_level l))
+        (decreases l)
+  =
+  match l with
+  | [] -> I.SNil
+  | hd::tl ->
+      let hd2 = to_node_inverse hd in
+      let tl2 = to_node_list_inverse_impl tl in
+      I.SCons hd2 tl2
+//---|
+
+
