src/study/Nemonuri.Study.CSharpSyntaxRewriter2.Modifier2/Nemonuri.StratifiedNodes.Nodes.Bijections.fst
@@ -1,0 +1,4 @@
+module Nemonuri.StratifiedNodes.Nodes.Bijections
+
+include Nemonuri.StratifiedNodes.Nodes.Bijections.ToNode
+include Nemonuri.StratifiedNodes.Nodes.Bijections.ToNodeList
